simplify the code with predicates and some comments, but still timeout on web Dafny

dafny/MergeSort.dfy
@@ -1,3 +1,12 @@
+//Proving merge sort
+//ISSUE: it be verified on local IDE, but it times out while verifying on website
+
+predicate permutation(a: seq<int>, b: seq<int>)
+{
+  if a == b then true else multiset(a) == multiset(b)
+}
+
+// To make Dafny know the elements in 2 subseq of a sequence is the same as the elements in this whole sequnce 
 lemma  MutisetAddingLemma(a: array<int>,l:int, m: int, u:int)
 requires 0<=l<=m<=u<a.Length
 ensures multiset(a[l..m]) + multiset(a[m..u+1]) == multiset(a[l..u+1])
@@ -5,9 +14,29 @@ ensures multiset(a[l..m]) + multiset(a[m..u+1]) == multiset(a[l..u+1])
     assert a[l..m] + a[m..u+1] == a[l..u+1];
 }
 
+predicate sortedBetween(a :array<int>, l : int, u : int)
+reads a;
+requires 0<=l <= u < a.Length
+{
+  forall q:: forall r:: l <= q < r <= u ==> a[q] <= a[r]
+}
+
+predicate ArraySorted(a :array<int>)
+reads a;
+{
+  forall q:: forall r:: 0 <= q < r < a.Length ==> a[q] <= a[r]
+}
+
+// //array a and b are equal int the range (0,l) and (u,a.Length) 
+// predicate Equivalence(a :array<int>, b: array<int>, l: int, u: int )
+// {
+
+// }
+
 method MergeSort(a1:array<int>) returns (a:array<int>)
   requires a1.Length > 0;
-  ensures forall k:: forall l:: 0 <= k < l < a.Length ==> a[k] <= a[l];
+  ensures ArraySorted(a);
+  ensures permutation(a[..], old(a)[..]);
 {
   a := mergesort(a1, 0, a1.Length-1);
   return;
@@ -18,27 +47,17 @@ method mergesort(a1:array<int>, l:int, u:int) returns (a:array<int>)
   requires 0 <= l <= u < a1.Length;
  
   ensures a.Length == a1.Length;
-  ensures forall q:: forall r:: l <= q < r <= u ==> a[q] <= a[r];
+  ensures sortedBetween(a,l,u);
   ensures forall q:: (0 <= q < l || u < q < a.Length) ==> a[q] == a1[q];
-  ensures multiset(a[l..u+1]) == multiset(a1[l..u+1]);
+  ensures permutation(a[l..u+1], a1[l..u+1]);
+  // ensures multiset(a[l..u+1]) == multiset(a1[l..u+1]);
   ensures a[0..l] == a1[0..l];
   ensures a[u+1..] == a1[u+1..];
   decreases u-l;
 {
   a := new int[a1.Length];
 
-    var o:= 0;
-  while (o < a.Length)
-    invariant a1.Length == a.Length
-    invariant 0 <= o <= a1.Length
-    invariant forall q:: (0 <= q < a.Length) ==> a1[q] == old(a1[q]);
-    invariant forall k:: 0 <= k < o ==> a[k] == a1[k]
-    invariant a1[0..o] == a[0..o]
-  {
-    a[o] := a1[o];
-    o := o + 1;
-  }
-  assert forall k:: 0 <= k < a1.Length ==> a[k] == a1[k];
+  copyArray(a1, a);
   if (l >= u)
   {
     return;
@@ -49,44 +68,51 @@ method mergesort(a1:array<int>, l:int, u:int) returns (a:array<int>)
     a := mergesort(a1, l, m);
     assert a[m+1..u+1] == a1[m+1..u+1];
     a := mergesort(a, m+1, u);
-    assert multiset(a[l..m+1]) == multiset(a1[l..m+1]);
-    assert multiset(a[m+1..u+1]) == multiset(a1[m+1..u+1]);
+
+    assert permutation(a[l..m+1], a1[l..m+1]);
+    assert permutation(a[m+1..u+1],a1[m+1..u+1]);
     MutisetAddingLemma(a,l,m+1,u);
     MutisetAddingLemma(a1,l,m+1,u);
     assert multiset(a[l..u+1]) == multiset(a1[l..u+1]);
+
     a := merge(a, l, m, u);
     return;
+  }
+}
+//this method copy array from a into b
+method copyArray(a: array<int>, b: array<int>)
+modifies b;
+requires a.Length  == b.Length
+ensures a.Length == b.Length
+ensures a[..] == b[..]
+ensures forall k:: 0 <= k < a.Length ==> a[k] == b[k];
+{
+  var o:= 0;
+  while (o < a.Length)
+    invariant 0 <= o <= a.Length
+    invariant forall q:: (0 <= q < a.Length) ==> a[q] == old(a[q]);
+    invariant b[0..o] == a[0..o]
+    invariant b.Length == a.Length
+  {
+    b[o] := a[o];
+    o := o + 1;
   }
 }
 
 method merge(a:array<int>, l:int, m:int, u:int) returns (buf:array<int>)
   requires a.Length > 0;
-  requires 0 <= l <= m <= u < a.Length;
-  requires forall q:: forall r:: l <= q < r <= m ==> a[q] <= a[r];
-  requires forall q:: forall r:: m+1 <= q < r <= u ==> a[q] <= a[r];
-  
+  requires 0 <= l <= m < u < a.Length;
+  requires sortedBetween(a,l,m);
+  requires sortedBetween(a,m+1,u);
   ensures a.Length == buf.Length;
   ensures multiset(buf[..]) == multiset(a[..]);
   ensures multiset(buf[l..u+1]) == multiset(a[l..u+1]);
-  ensures forall q:: forall r:: l <= q < r <= u ==> buf[q] <= buf[r];
+  ensures sortedBetween(buf,l,u);
   ensures forall q:: (0 <= q < l || u < q < buf.Length) ==> buf[q] == a[q];
 {
-//   var a := new int[a.Length];
-//   assume forall k:: 0 <= k < a.Length ==> a[k] == a[k];
-  
+
   buf := new int[a.Length];
-  var o:= 0;
-  while (o < a.Length)
-    invariant buf.Length == a.Length
-    invariant 0 <= o <= a.Length
-    invariant forall q:: (0 <= q < a.Length) ==> a[q] == old(a[q]);
-    invariant forall k:: 0 <= k < o ==> a[k] == buf[k]
-    invariant buf[0..o] == a[0..o]
-  {
-    buf[o] := a[o];
-    o := o + 1;
-  }
-  assert forall k:: 0 <= k < a.Length ==> a[k] == buf[k];
+  copyArray(a, buf);
 
 
   var i:int := l;
@@ -101,10 +127,10 @@ method merge(a:array<int>, l:int, m:int, u:int) returns (buf:array<int>)
     
     invariant (i-l) + (j-(m+1)) == k; // k aligns properly.
     invariant buf.Length == a.Length;
-    invariant multiset(buf[l..l+k]) == multiset(a[l..i]) + multiset(a[m+1..j]);
+    invariant multiset(buf[l..l+k]) == multiset(a[l..i]) + multiset(a[m+1..j]);  // elements maintain the same
     invariant buf[0..l] == a[0..l];
     invariant buf[u+1..] == a[u+1..];
-    invariant forall q:: forall r:: l <= q < r < k+l ==>  buf[q] <= buf[r]; // buf is sorted in [0,k). Most important condition.
+    invariant forall q:: forall r:: l <= q < r <= k+l-1 ==>  buf[q] <= buf[r]; // buf is sorted in [l,k+l].
     invariant forall q:: forall r:: l <= q < l+k && (i <= r <= m || j <= r <= u) ==> buf[q] <= a[r];
 
   {
@@ -130,24 +156,24 @@ method merge(a:array<int>, l:int, m:int, u:int) returns (buf:array<int>)
     }
     k := k + 1;
   }
-  assert j == u+1;
-  assert i == m+1;
-  assert k==u-l+1;
-//   assert multiset(buf[..buf.Length]) == multiset(a[l..i]) + multiset(a[m+1..j]);
-//   assert buf[..buf.Length] == buf[..];
-  assert multiset(buf[l..u+1]) == multiset(a[l..m+1]) + multiset(a[m+1..u+1]);
-  assert a[l..m+1] + a[m+1..u+1] == a[l..u+1];
-assert multiset(a[l..m+1]) + multiset(a[m+1..u+1]) == multiset(a[l..u+1]);
-  assert  buf[0..l] + buf[l..u+1] + buf[u+1..] == buf[..];
-    assert buf[0..l] == a[0..l];
-    assert buf[u+1..] == a[u+1..];
-  assert  a[0..l] + a[l..u+1] + a[u+1..] == a[..];
-
-    assert multiset(buf[u+1..]) == multiset(a[u+1..]);
-    assert multiset(buf[0..l]) == multiset(a[0..l]);
-  assert multiset(buf[l..u+1]) == multiset(a[l..u+1]);
+  // assert j == u+1;
+  // assert i == m+1;
+  // assert k==u-l+1;
+  MutisetAddingLemma(buf,l,m+1,u);
+  MutisetAddingLemma(a,l,m+1,u);
+  // assert multiset(buf[l..u+1]) == multiset(a[l..m+1]) + multiset(a[m+1..u+1]);
+  // assert a[l..m+1] + a[m+1..u+1] == a[l..u+1];
+  // assert multiset(a[l..m+1]) + multiset(a[m+1..u+1]) == multiset(a[l..u+1]);
+    // assert buf[0..l] == a[0..l];
+    // assert buf[u+1..] == a[u+1..];
+  assert  buf[..l] + buf[l..u+1] + buf[u+1..] == buf[..];
+  assert  a[..l] + a[l..u+1] + a[u+1..] == a[..];
   assert multiset(buf[0..l]) + multiset(buf[l..u+1]) + multiset(buf[u+1..]) == multiset(buf[..]);
   assert multiset(a[0..l]) + multiset(a[l..u+1]) + multiset(a[u+1..]) == multiset(a[..]);
+
+  assert multiset(buf[u+1..]) == multiset(a[u+1..]);
+  assert multiset(buf[0..l]) == multiset(a[0..l]);
+  assert multiset(buf[l..u+1]) == multiset(a[l..u+1]);
   assert multiset(buf[..]) == multiset(a[..]);
 
 }
